Ye olde pile of redexes

DeBruijnSSA/BinSyntax/Rewrite.lean
@@ -18,44 +18,118 @@ def Term.WfD.subst₂ {Γ : Ctx α ε} {a b : Term φ}
   | ⟨1, _⟩ => hb
   | ⟨n + 2, h⟩ => var ⟨by simp at h; exact h, le_refl _⟩
 
-inductive Region.Beta (Γ : Ctx α ε) : Region φ → Region φ → Prop
+inductive Region.CBeta (Γ : Ctx α ε) : Region φ → Region φ → Prop
   | let1 (e : Term φ) (r : Region φ)
-    : e.infEffect Γ = ⊥ → Beta Γ (r.let1 e) (r.vsubst e.subst0)
-  | let2 (a : Term φ) (b : Term φ) (r : Region φ)
-    : a.infEffect Γ = ⊥ → b.infEffect Γ = ⊥ → Beta Γ (r.let2 (a.pair b)) (r.vsubst (a.subst₂ b))
-  | case_left (e : Term φ) (r : Region φ) (s : Region φ) : Beta Γ (case e.inl r s) (let1 e r)
-  | case_right (e : Term φ) (r : Region φ) (s : Region φ) : Beta Γ (case e.inr r s) (let1 e s)
+    : e.infEffect Γ = ⊥ → CBeta Γ (r.let1 e) (r.vsubst e.subst0)
 
-theorem Region.Beta.let1_pure {Γ : Ctx α ε} {e} {r r' : Region φ}
-  (h : Region.Beta Γ (r.let1 e) r') : e.infEffect Γ = ⊥ := by cases h; assumption
+theorem Region.CBeta.let1_pure {Γ : Ctx α ε} {e} {r r' : Region φ}
+  (h : Region.CBeta Γ (r.let1 e) r') : e.infEffect Γ = ⊥ := by cases h; assumption
 
-theorem Region.Beta.let1_trg {Γ : Ctx α ε} {e} {r r' : Region φ}
-  (h : Region.Beta Γ (r.let1 e) r') : r' = r.vsubst e.subst0 := by cases h; rfl
+theorem Region.CBeta.let1_trg {Γ : Ctx α ε} {e} {r r' : Region φ}
+  (h : Region.CBeta Γ (r.let1 e) r') : r' = r.vsubst e.subst0 := by cases h; rfl
 
-theorem Region.Beta.let2_left_pure {Γ : Ctx α ε} {a b : Term φ} {r r' : Region φ}
-  (h : Region.Beta Γ (r.let2 (a.pair b)) r') : a.infEffect Γ = ⊥ := by cases h; assumption
-
-theorem Region.Beta.let2_right_pure {Γ : Ctx α ε} {a b : Term φ} {r r' : Region φ}
-  (h : Region.Beta Γ (r.let2 (a.pair b)) r') : b.infEffect Γ = ⊥ := by cases h; assumption
-
-theorem Region.Beta.let2_trg {Γ : Ctx α ε} {a b : Term φ} {r r' : Region φ}
-  (h : Region.Beta Γ (r.let2 (a.pair b)) r') : r' = r.vsubst (a.subst₂ b) := by cases h; rfl
-
-theorem Region.Beta.case_left_trg {Γ : Ctx α ε} {e} {r s r' : Region φ}
-  (h : Region.Beta Γ (case e.inl r s) r') : r' = r.let1 e := by cases h; rfl
-
-theorem Region.Beta.case_right_trg {Γ : Ctx α ε} {e} {r s s' : Region φ}
-  (h : Region.Beta Γ (case e.inr r s) s') : s' = s.let1 e := by cases h; rfl
-
-def Region.Beta.WfD {Γ : Ctx α ε} {r r' : Region φ}
-  : Region.Beta Γ r r' → r.WfD Γ A → r'.WfD Γ A
+def Region.CBeta.WfD {Γ : Ctx α ε} {r r' : Region φ}
+  : Region.CBeta Γ r r' → r.WfD Γ A → r'.WfD Γ A
   | h, WfD.let1 de dr => h.let1_trg ▸ dr.vsubst (h.let1_pure ▸ de.toInfEffect.subst0)
-  | h, WfD.let2 (Term.WfD.pair da db) dr => h.let2_trg ▸
-    dr.vsubst ((h.let2_left_pure ▸ da.toInfEffect).subst₂ (h.let2_right_pure ▸ db.toInfEffect))
-  | h, WfD.case (Term.WfD.inl de) dr _ => h.case_left_trg ▸ dr.let1 de
-  | h, WfD.case (Term.WfD.inr de) _ ds => h.case_right_trg ▸ ds.let1 de
 
--- inductive Region.FuseLet (Γ : Ctx α ε) : Region φ → Region φ → Region φ → Prop
---   | fuse (e : Term φ) (r : Region φ) (s : Region φ)
+inductive Region.Reduce : Region φ → Region φ → Prop
+  | let2_pair (a b r) : Reduce (let2 (Term.pair a b) r) (let1 a $ let1 (b.wk Nat.succ) $ r)
+  | case_inl (e r s) : Reduce (case (Term.inl e) r s) (let1 e r)
+  | case_inr (e r s) : Reduce (case (Term.inr e) r s) (let1 e s)
+
+theorem Region.Reduce.let2_pair_trg {a b} {r r' : Region φ}
+  (h : Region.Reduce (Region.let2 (Term.pair a b) r) r')
+  : r' = (Region.let1 a $ Region.let1 (b.wk Nat.succ) $ r) := by cases h; rfl
+
+theorem Region.Reduce.case_inl_trg {e} {r s r' : Region φ}
+  (h : Region.Reduce (Region.case (Term.inl e) r s) r')
+  : r' = (Region.let1 e r) := by cases h; rfl
+
+theorem Region.Reduce.case_inr_trg {e} {r s s' : Region φ}
+  (h : Region.Reduce (Region.case (Term.inr e) r s) s')
+  : s' = (Region.let1 e s) := by cases h; rfl
+
+def Region.Reduce.WfD {Γ : Ctx α ε} {r r' : Region φ}
+  : Region.Reduce r r' → r.WfD Γ A → r'.WfD Γ A
+  | h, WfD.let2 (Term.WfD.pair da db) dr
+    => h.let2_pair_trg ▸ (WfD.let1 da $ WfD.let1 (db.wk ((Ctx.Wkn.id _).step)) $ dr)
+  | h, WfD.case (Term.WfD.inl de) dr _ => h.case_inl_trg ▸ dr.let1 de
+  | h, WfD.case (Term.WfD.inr de) _ ds => h.case_inr_trg ▸ ds.let1 de
+
+inductive Region.TermEta1 : Region φ → Region φ → Prop
+  | let1_op (f e r) : TermEta1 (let1 (Term.op f e) r)
+    (let1 e
+      $ let1 (Term.op f (Term.var 0))
+      $ r.vwk (Nat.liftWk Nat.succ))
+  | let1_pair (a b r) : TermEta1 (let1 (Term.pair a b) r)
+    (let1 a
+      $ let1 b
+      $ let1 (Term.pair (Term.var 1) (Term.var 0))
+      $ r.vwk (Nat.liftWk (· + 2))
+    )
+  | let1_inl (e r s) : TermEta1 (case (Term.inl e) r s)
+    (let1 e
+      $ let1 (Term.inl (Term.var 0))
+      $ r.vwk (Nat.liftWk Nat.succ))
+  | let1_inr (e r s) : TermEta1 (case (Term.inr e) r s)
+    (let1 e
+      $ let1 (Term.inr (Term.var 0))
+      $ s.vwk (Nat.liftWk Nat.succ))
+  | let1_abort (e r) : TermEta1 (let1 (Term.abort e) r)
+    (let1 e
+      $ let1 (Term.abort (Term.var 0))
+      $ r.vwk (Nat.liftWk Nat.succ))
+
+-- TODO: WfD preservation for TermEta1
+
+inductive Region.TermEta2 : Region φ → Region φ → Prop
+  | let2_op (f e r) : TermEta2 (let2 (Term.op f e) r) (let1 e
+      $ let2 (Term.op f (Term.var 0))
+      $ r.vwk (Nat.liftnWk 2 Nat.succ))
+
+-- TODO: WfD preservation for TermEta2
+
+inductive Region.Eta : Region φ → Region φ → Prop
+  | let1_case (a b r s) : Eta
+    (let1 a $ case (b.wk Nat.succ) r s)
+    (case b (let1 (a.wk Nat.succ) r) (let1 (a.wk Nat.succ) s))
+  | let2_case (a b r s) : Eta
+    (let2 a $ case (b.wk (· + 2)) r s)
+    (case b (let2 (a.wk Nat.succ) r) (let2 (a.wk Nat.succ) s))
+  | cfg_br_lt (ℓ e n G) (h : ℓ < n) : Eta
+    (cfg (br ℓ e) n G)
+    (cfg ((G ⟨ℓ, h⟩).vsubst e.subst0) n G)
+  | cfg_br_ge (ℓ e n G) (h : n ≤ ℓ) : Eta
+    (cfg (br ℓ e) n G)
+    (cfg (br (ℓ - n) e) n G)
+  | cfg_let1 (a β n G) : Eta
+    (cfg (let1 a β) n G)
+    (let1 a $ cfg β n (vwk Nat.succ ∘ G))
+  | cfg_let2 (a β n G) : Eta
+    (cfg (let2 a β) n G)
+    (let2 a $ cfg β n (vwk (· + 2) ∘ G))
+  | cfg_case (e r s n G) : Eta
+    (cfg (case e r s) n G)
+    (case e (cfg r n (vwk Nat.succ ∘ G)) (cfg s n (vwk Nat.succ ∘ G)))
+  | cfg_cfg (β n G n' G') : Eta
+    (cfg (cfg β n G) n' G')
+    (cfg β (n' + n) (Fin.addCases (lwk (· + n) ∘ G') G))
+
+inductive Region.WkCfg : Region φ → Region φ → Prop
+  | cfg (β n G k) (ρ : Fin k → Fin n)
+    : WkCfg (cfg (β.lwk (Fin.toNatWk ρ)) n G) (cfg β k (G ∘ ρ))
+
+-- TODO: general eta...
+
+inductive Region.SimpleCongruence (P : Region φ → Region φ → Prop) : Region φ → Region φ → Prop
+  | step (r r') : P r r' → SimpleCongruence P r r'
+  | let1 (e r r') : SimpleCongruence P r r' → SimpleCongruence P (let1 e r) (let1 e r')
+  | let2 (e r r') : SimpleCongruence P r r' → SimpleCongruence P (let2 e r) (let2 e r')
+  | case_left (e r s r') : SimpleCongruence P r r' → SimpleCongruence P (case e r s) (case e r' s)
+  | case_right (e r s s') : SimpleCongruence P s s' → SimpleCongruence P (case e r s) (case e r s')
+  | cfg_entry (r r' n G) : SimpleCongruence P r r' → SimpleCongruence P (cfg r n G) (cfg r' n G)
+  | cfg_block (r r' n G i G') : SimpleCongruence P r r' → G' = Function.update G i r' →
+    SimpleCongruence P (cfg β n G) (cfg β n G')
+
 
 end BinSyntax
